

Mat 2540 HW2

1. Find $f(1)$, $f(2)$, $f(3)$, and $f(4)$ if $f(n)$ is defined recursively

by $f(0) = 1$ and for $n = 0, 1, 2, \dots$

a) $f(n+1) = f(n) + 2$.

b) $f(n+1) = 3f(n)$.

c) $f(n+1) = 2^{f(n)}$.

d) $f(n+1) = f(n)^2 + f(n) + 1$.

Sol: a) $n=0$, $f(1) = f(0+1) = f(0) + 2 = 1 + 2 = 3$

$n=1$, $f(2) = f(1+1) = f(1) + 2 = 3 + 2 = 5$

$n=2$, $f(3) = f(2+1) = f(2) + 2 = 5 + 2 = 7$

$n=3$, $f(4) = f(3+1) = f(3) + 2 = 7 + 2 = 9$

b) $n=0$, $f(1) = f(0+1) = 3 \cdot f(0) = 3 \cdot 1 = 3$

$n=1$, $f(2) = f(1+1) = 3 \cdot f(1) = 3 \cdot 3 = 9$

$n=2$, $f(3) = f(2+1) = 3 \cdot f(2) = 3 \cdot 9 = 27$

$n=3$, $f(4) = f(3+1) = 3 \cdot f(3) = 3 \cdot 27 = 81$

c) $n=0$, $f(1) = f(0+1) = 2^{f(0)} = 2^1 = 2$

$n=1$, $f(2) = f(1+1) = 2^{f(1)} = 2^2 = 4$

$n=2$, $f(3) = f(2+1) = 2^{f(2)} = 2^4 = 16$

$n=3$, $f(4) = f(3+1) = 2^{f(3)} = 2^{16}$

d) $n=0$, $f(1) = f(0+1) = f(0)^2 + f(0) + 1 = 1^2 + 1 + 1 = 3$

$n=1$, $f(2) = f(1+1) = f(1)^2 + f(1) + 1 = 3^2 + 3 + 1 = 13$

$n=2$, $f(3) = f(2+1) = f(2)^2 + f(2) + 1 = 13^2 + 13 + 1 = 183$

$n=3$, $f(4) = f(3+1) = f(3)^2 + f(3) + 1 = 183^2 + 183 + 1$

3. Find $f(2)$, $f(3)$, $f(4)$, and $f(5)$ if f is defined recursively

by $f(0) = -1$, $f(1) = 2$, and for $n = 1, 2, \dots$

a) $f(n+1) = f(n) + 3f(n-1)$.

b) $f(n+1) = f(n)^2 f(n-1)$.

c) $f(n+1) = 3f(n)^2 - 4f(n-1)^2$.

d) $f(n+1) = f(n-1)/f(n)$.

a) $n=1$, $f(2) = f(1+1) = f(1) + 3f(0) = 2 + 3 \cdot (-1) = -1$

$n=2$, $f(3) = f(2+1) = f(2) + 3f(1) = (-1) + 3 \cdot 2 = 5$

$n=3$, $f(4) = f(3+1) = f(3) + 3f(2) = 5 + 3 \cdot (-1) = 2$

$n=4$, $f(5) = f(4+1) = f(4) + 3f(3) = 2 + 3 \cdot 5 = 17$

$$b) n=1, f(2)=f(1+1)=f(1)^2 \cdot f(0) = 2^2 \cdot (-1) = -4$$

$$n=2, f(3)=f(2+1)=f(2)^2 \cdot f(1) = (-4)^2 \cdot 2 = 32$$

$$n=3, f(4)=f(3+1)=f(3)^2 \cdot f(2) = (32)^2 \cdot (-4) = -4096$$

$$n=4, f(5)=f(4+1)=f(4)^2 \cdot f(3) = (-4096)^2 \cdot 32 = 2^{29}$$

$$c) n=1, f(2)=f(1+1)=3f(1)^2-4f(0)^2 = 3(2)^2-4(-1)^2 = 8$$

$$n=2, f(3)=f(2+1)=3f(2)^2-4f(1)^2 = 3(8)^2-4(2)^2 = 176$$

$$n=3, f(4)=f(3+1)=3f(3)^2-4f(2)^2 = 3(176)^2-4(8)^2 = 92672$$

$$n=4, f(5)=f(4+1)=3f(4)^2-4f(3)^2 = 3(92672)^2-4(176)^2$$

$$d) n=1, f(2)=f(1+1)=\frac{f(1)}{f(0)} = \frac{-1}{2} = -\frac{1}{2}$$

$$n=2, f(3)=f(2+1)=\frac{f(2)}{f(1)} = \frac{-\frac{1}{2}}{-1} = \frac{1}{2}$$

$$n=3, f(4)=f(3+1)=\frac{f(3)}{f(2)} = \frac{\frac{1}{2}}{-\frac{1}{2}} = -1$$

$$n=4, f(5)=f(4+1)=\frac{f(4)}{f(3)} = \frac{-1}{\frac{1}{2}} = -2$$

5. Determine whether each of these proposed definitions is a valid recursive definition of a function f from the set of nonnegative integers to the set of integers. If f is well defined, find a formula for $f(n)$ when n is a nonnegative integer and prove that your formula is valid.

a) $f(0) = 0, f(n) = 2f(n-2)$ for $n \geq 1$

b) $f(0) = 1, f(n) = f(n-1) - 1$ for $n \geq 1$

c) $f(0) = 2, f(1) = 3, f(n) = f(n-1) - 1$ for $n \geq 2$

d) $f(0) = 1, f(1) = 2, f(n) = 2f(n-2)$ for $n \geq 2$

e) $f(0) = 1, f(n) = 3f(n-1)$ if n is odd and $n \geq 1$ and $f(n) = 9f(n-2)$ if n is even and $n \geq 2$

a) When $n=1$, we have $f(1)=2f(1-2)=2f(-1)$.

However, we don't know $f(-1)$. Thus, this is NOT a valid one.

b) $f(1)=f(1-1)-1=f(0)-1=1-1=0$
 $f(2)=f(2-1)-1=f(1)-1=0-1=-1$
 $f(3)=f(3-1)-1=f(2)-1=-1-1=-2$
 $f(4)=f(4-1)-1=f(3)-1=-2-1=-3$
 \vdots

Assume

$$f(n)=1+n \cdot (-1) \quad n \geq 1$$

Proof: $f(n)=f(n-1)-1 \Rightarrow f(n)-f(n-1)=-1$ and it means that

there is a common difference $d=-1$ from previous term to the

current term, and $f(n)$ is an arithmetic sequence with initial term $f(0)=1$

Thus, the exact formula of $f(n)$ is

$$f(n) = f(0) + n \cdot d = 1 + n \cdot (-1) \quad \text{for } n \geq 1$$

c) $f(0)=2, f(1)=3, f(n)=f(n-1)-1$ for $n \geq 2$

Since $f(n)=f(n-1)-1$, we have $f(n)-f(n-1)=-1$, which means

$f(n)$ is an arithmetic sequence with common difference $d=-1$

with $f(0)=2, f(1)=3$.

Therefore, we have $f(n) = 3 + (n-1)(-1) = 3+1-n = 4-n$ for $n \geq 1$ and $f(0)=2$

Prove $f(n)=4-n$ for $n \geq 1$ by induction, we have

Basis step: $f(1)=4-1=3$ and given $f(0)=2$.

Inductive step: Assume $f(k)=4-k$ for $k \geq 1$. To prove $f(k+1)=4-(k+1)$.

$$\text{We have } f(k+1) = f(k) - 1 = 4 - k - 1 = 4 - (k+1)$$

which shows $f(k+1)=4-(k+1)$ is true and

$$f(n) = 4 - n, \quad n \geq 1 \quad \text{and} \quad f(0)=2.$$

d) Given $f(0)=1, f(1)=2, f(n)=2f(n-2), n \geq 2$. We have

$$f(0)=1, f(1)=2$$

$$f(2)=2 \cdot f(2-2) = 2 \cdot f(0) = 2 \cdot 1 = 2 = 2^1$$

$$f(3)=2 \cdot f(3-2) = 2 \cdot f(1) = 2 \cdot 2 = 4 = 2^2 \Rightarrow$$

$$f(4)=2 \cdot f(4-2) = 2 \cdot f(2) = 2 \cdot 2 = 4 = 2^2$$

$$f(5)=2 \cdot f(5-2) = 2 \cdot f(3) = 2 \cdot 4 = 8 = 2^3$$

To prove $f(n) = 2^{\lfloor \frac{n+1}{2} \rfloor}$ for $n \geq 0$ by ^{strong} induction, we have

$$\text{Basis Step: } f(0) = 2^{\lfloor \frac{0+1}{2} \rfloor} = 2^0 = 1 \quad (\text{checked})$$

$$f(1) = 2^{\lfloor \frac{1+1}{2} \rfloor} = 2^1 = 2 \quad (\text{checked})$$

Inductive step: Assume $f(j) = 2^{\lfloor \frac{j+1}{2} \rfloor}$ for $0 \leq j \leq k$ with $k \geq 1$.

Assume $f(n) = 2^{\lfloor \frac{n+1}{2} \rfloor}, n \geq 0$

^{floor function}

To prove $f(k+1) = 2^{\lfloor \frac{k+1+1}{2} \rfloor}$, we have
 $k \geq 1 \Rightarrow k-1 \geq 0$ and $f(k-1) = 2^{\lfloor \frac{(k-1)+1}{2} \rfloor} = 2^{\lfloor \frac{k}{2} \rfloor}$.

Then, by the original formula,

$$f(k+1) = 2 \cdot f(k-1) = 2 \cdot 2^{\lfloor \frac{k}{2} \rfloor} = 2^{\lfloor \frac{k}{2} \rfloor + 1} = 2^{\lfloor \frac{k}{2} + 1 \rfloor}$$

$$\text{By strong induction, } f(n) = 2^{\lfloor \frac{n+1}{2} \rfloor}, n \geq 0. \quad (= 2^{\lfloor \frac{k+2}{2} \rfloor} = 2^{\lfloor \frac{(k+1)+1}{2} \rfloor} \text{ (checked)})$$

e) Given $f(0) = 1$, $f(n) = \begin{cases} 3 \cdot f(n-1) & , n \text{ is odd and } n \geq 1 \\ 9 \cdot f(n-2) & , n \text{ is even and } n \geq 2 \end{cases}$

$$f(1) = 3 \cdot f(0) = 3 \cdot 1 = 3 = 3^1$$

$$f(2) = 9 \cdot f(0) = 9 \cdot 1 = 9 = 3^2$$

$$f(3) = 3 \cdot f(2) = 3 \cdot 9 = 27 = 3^3 \Rightarrow \text{Assume } f(n) = 3^n, n \geq 0.$$

$$f(4) = 9 \cdot f(2) = 9 \cdot 9 = 81 = 3^4$$

$$f(5) = 3 \cdot f(4) = 3 \cdot 81 = 3^5$$

To prove $f(n) = 3^n, n \geq 0$ by strong induction, we have

Basis step: $f(0) = 3^0 = 1$ (checked)

$$f(1) = 3 \cdot f(0) = 3 = 3^1 \text{ (checked)}$$

$$f(2) = 9 \cdot f(0) = 9 = 3^2 \text{ (checked)}$$

Inductive step: Assume $f(j) = 3^j$ for $0 \leq j \leq k, k \geq 2$.

To prove $f(k+1) = 3^{k+1}, k+1 \geq 3$ we have two cases:

① If $k+1$ is odd, then

$$f(k+1) = 3 \cdot f(k) = 3 \cdot 3^k = 3^{k+1}$$

② If $k+1$ is even, then $k-1 \geq 1$

$$f(k+1) = 9 \cdot f(k-1) = 9 \cdot 3^{k-1} = 3^{k+1}$$

By strong induction, $f(n) = 3^n$ for $n \geq 0$.

7. Give a recursive definition of the sequence $\{a_n\}$, $n = 1, 2, 3, \dots$ if

- a) $a_n = 6n$.
c) $a_n = 10^n$.

- b) $a_n = 2n + 1$.
d) $a_n = 5$.

a) Given $a_n = 6n$, $a_1, a_2, a_3, a_4, \dots, a_n, a_{n+1}$
 $\begin{array}{ccccccc} a_1 & a_2 & a_3 & a_4 & \dots & a_n & a_{n+1} \\ \parallel & \parallel & \parallel & \parallel & & \parallel & \parallel \\ 6 & 6 \cdot 2 & 6 \cdot 3 & 6 \cdot 4 & & 6 \cdot n & 6(n+1) \\ \parallel & \parallel & \parallel & \parallel & & \parallel & \parallel \\ & 12 & 18 & 24 & & & \end{array}$
 $a_2 - a_1 = 6, a_3 - a_2 = 6, a_4 - a_3 = 6, \dots, a_{n+1} - a_n = 6$

$\Rightarrow a_{n+1} = a_n + 6$ with $a_1 = 6, n \geq 1$

b) $a_n = 2n + 1$, $a_1, a_2, a_3, a_4, \dots, a_n, a_{n+1}$
 $\begin{array}{ccccccc} a_1 & a_2 & a_3 & a_4 & \dots & a_n & a_{n+1} \\ \parallel & \parallel & \parallel & \parallel & & \parallel & \parallel \\ 2 \cdot 1 + 1 & 2 \cdot 2 + 1 & 2 \cdot 3 + 1 & 2 \cdot 4 + 1 & & 2 \cdot n + 1 & 2(n+1) + 1 \\ \parallel & \parallel & \parallel & \parallel & & \parallel & \parallel \\ & 3 & 5 & 7 & & 9 & \end{array}$
 $a_2 - a_1 = 2, a_3 - a_2 = 2, a_4 - a_3 = 2, \dots, a_{n+1} - a_n = 2$

$\Rightarrow a_{n+1} = a_n + 2, n \geq 1$ with $a_1 = 3$

c) $a_n = 10^n$, $a_1, a_2, a_3, a_4, \dots, a_n, a_{n+1}$
 $\begin{array}{ccccccc} a_1 & a_2 & a_3 & a_4 & \dots & a_n & a_{n+1} \\ \parallel & \parallel & \parallel & \parallel & & \parallel & \parallel \\ 10^1 & 10^2 & 10^3 & 10^4 & & 10^n & 10^{n+1} \\ \parallel & \parallel & \parallel & \parallel & & \parallel & \parallel \\ & 10 & 100 & 1000 & & & \end{array}$
 $\frac{a_2}{a_1} = 10, \frac{a_3}{a_2} = 10, \frac{a_4}{a_3} = 10, \dots, \frac{a_{n+1}}{a_n} = 10$

$\Rightarrow a_{n+1} = 10 \cdot a_n, n \geq 1$ with $a_1 = 10$

d) $a_n = 5$, $a_1, a_2, a_3, \dots, a_n, a_{n+1}$
 $\begin{array}{ccccccc} a_1 & a_2 & a_3 & \dots & a_n & a_{n+1} \\ \parallel & \parallel & \parallel & & \parallel & \parallel \\ 5 & 5 & 5 & & 5 & 5 \\ \parallel & \parallel & \parallel & & \parallel & \parallel \\ & 5 & 5 & & 5 & 5 \end{array}$
 $a_2 = a_1, a_3 = a_2, \dots, a_{n+1} = a_n$
 $\Rightarrow a_{n+1} = a_n, n \geq 1$ with $a_1 = 5$.

9. Let F be the function such that $F(n)$ is the sum of the first n positive integers. Give a recursive definition of $F(n)$.

Given $F(n) = \sum_{k=1}^n k$, we have

$F(1) = 1, F(2) = 1+2 = 3, F(3) = 1+2+3 = 6, \dots, F(n) = 1+2+\dots+n, F(n+1) = 1+2+\dots+n+(n+1)$

$\Rightarrow F(n+1) = F(n) + (n+1)$ with $F(1) = 1$ and $n \geq 1$

* 20. Give a recursive definition of the functions max and min so that $\max(a_1, a_2, \dots, a_n)$ and $\min(a_1, a_2, \dots, a_n)$ are the maximum and minimum of the n numbers a_1, a_2, \dots, a_n , respectively.

① If there is only 1 element, the max or min value is itself.

② If there are 2 elements, denoted by a_1, a_2 , then

$$\max(a_1, a_2) = \begin{cases} a_1 & , a_1 \geq a_2 \\ a_2 & , a_2 > a_1 \end{cases}$$

③ If there are $n+1$ elements, we have

$$\max(a_1, a_2, a_3, \dots, a_n, a_{n+1}) = \max(\max(a_1, a_2, \dots, a_n), a_{n+1})$$

(Similarly, $\min(a_1, a_2, a_3, \dots, a_n, a_{n+1}) = \min(\min(a_1, a_2, \dots, a_n), a_{n+1})$)